wip: progress

tests/playground/int_exhaust_test.lean
@@ -7,12 +7,14 @@ open Lean.Elab.Command (CommandElab)
 open Lean.Test.NormalForms
 
 inductive NumType where
+  | prop
   | nat
   | int
 deriving DecidableEq, Hashable, Inhabited, Repr
 
 protected def NumType.render [Monad M] [MonadQuotation M] (v : NumType) : M Term := do
   match v with
+  | prop => `(Prop)
   | nat => `(Nat)
   | int => `(Int)
 
@@ -35,14 +37,17 @@ def DivMode.typeOf (m : DivMode) : NumType :=
 inductive NumTerm where
   | var (d : VarDecl NumType)
   | lit (n : Nat) (tp : NumType)
-  | natToInt (x : NumTerm)
-  | intToNat (x : NumTerm)
+  | natCast (x : NumTerm)
   | add (x y : NumTerm) (tp : NumType)
   | sub (x y : NumTerm) (tp : NumType)
   | neg (x : NumTerm)
   | mul (x y : NumTerm) (tp : NumType)
   | div (x y : NumTerm) (m : DivMode)
   | mod (x y : NumTerm) (m : DivMode)
+  | eq (x y : NumTerm) (tp : NumType)
+  | le (x y : NumTerm) (tp : NumType)
+  | lt (x y : NumTerm) (tp : NumType)
+  | true | false
   deriving BEq, Inhabited, Repr
 
 namespace NumTerm
@@ -52,38 +57,38 @@ open NumType
 partial def map (f : NumTerm → NumTerm) (v : NumTerm) : NumTerm :=
   match v with
   | var _ | lit _ _ => v
-  | natToInt x => natToInt (f x)
-  | intToNat x => intToNat (f x)
+  | natCast x => natCast (f x)
   | add x y tp => add (f x) (f y) tp
   | sub x y tp => sub (f x) (f y) tp
   | neg x => neg (f x)
   | mul x y tp => mul (f x) (f y) tp
   | div x y op => div (f x) (f y) op
   | mod x y op => mod (f x) (f y) op
+  | eq x y tp => eq (f x) (f y) tp
+  | le x y tp => le (f x) (f y) tp
+  | lt x y tp => lt (f x) (f y) tp
+  | true => true
+  | false => false
 
 protected def typeOf (v : NumTerm) : NumType :=
   match v with
   | var d => d.type
   | lit _ tp => tp
-  | natToInt _ => .int
-  | intToNat _ => .nat
-  | add _ _ tp => tp
-  | sub _ _ tp => tp
+  | natCast _ => .int
+  | add _ _ tp | sub _ _ tp | mul _ _ tp => tp
   | neg _ => .int
-  | mul _ _ tp => tp
-  | div _ _ op => op.typeOf
-  | mod _ _ op => op.typeOf
+  | div _ _ op | mod _ _ op => op.typeOf
+  | eq .. | le .. | lt .. | true | false => .prop
 
 protected def render [Monad M] [MonadQuotation M] (v : NumTerm) : M Term := do
   match v with
   | var d => pure d.ident
-  | lit n tp => `(($(Syntax.mkNumLit (toString n)) : $(←tp.render)))
-  | natToInt x => `((($(←x.render) : Nat) : Int))
-  | intToNat x => `((($(←x.render) : Int) : Nat))
-  | add x y tp => `((($(←x.render) + $(←y.render)) : $(←tp.render)))
-  | sub x y _ => `($(←x.render) - $(←y.render))
+  | lit n tp => `(($(Syntax.mkNumLit (toString n)) : $(← tp.render)))
+  | natCast x => `(($(←x.render).cast : Int))
+  | add x y tp => `((($(←x.render) + $(←y.render)) : $(← tp.render)))
+  | sub x y tp => `((($(←x.render) - $(←y.render)) : $(← tp.render)))
+  | mul x y tp => `((($(←x.render) * $(←y.render)) : $(← tp.render)))
   | neg x => `(- $(←x.render))
-  | mul x y _ => `($(←x.render) * $(←y.render))
   | div x y op =>
     match op with
     | .divNat  => `($(←x.render) / $(←y.render))
@@ -98,6 +103,11 @@ protected def render [Monad M] [MonadQuotation M] (v : NumTerm) : M Term := do
     | .fdivInt => `(Int.fmod $(←x.render) $(←y.render))
     | .tdivInt => `(Int.mod  $(←x.render) $(←y.render))
     | .bdivInt => `(Int.bmod $(←x.render) $(←y.render))
+  | eq x y _ => `($(←x.render) = $(←y.render))
+  | le x y _ => `($(←x.render) ≤ $(←y.render))
+  | lt x y _ => `($(←x.render) < $(←y.render))
+  | true => `(True)
+  | false => `(False)
 
 instance : GenTerm NumTerm NumType where
   render := NumTerm.render
@@ -109,9 +119,12 @@ def intLit (i : Int) : NumTerm :=
   else
     lit i.toNat .int
 
+def mkConstProp (b : Bool) : NumTerm := cond b .true .false
+
 def mkLit (i : Int) (tp : NumType) : NumTerm :=
   if i < 0 then
     match tp with
+    | .prop => panic! "prop literal not allowed"
     | .nat => panic! "Negative number passed into nat"
     | .int => neg (lit ((- i).toNat) .int)
   else
@@ -123,17 +136,33 @@ def asIntLit (i : NumTerm) : Option Int :=
   | .neg (.lit n .int) => some (- (n : Int))
   | _ => none
 
+/--
+Returns nat term or literal equal to input term if input
+term is a literal or has form `natToInt _`.
+-/
+def intAtNat (x : NumTerm) : Option NumTerm :=
+  match x with
+  | lit xn .int => some (lit xn .nat)
+  | natCast x => some x
+  | _ => none
+
+def isPos (x : NumTerm) : Bool :=
+  match x with
+  | lit xn .nat => xn > 0
+  | _ => Bool.false
+
 partial def simp (v : NumTerm) : NumTerm :=
   let v := map simp v
   match v with
-  | natToInt x =>
+  | natCast x =>
     (match x with
     | lit n _ => lit n .int
-    | add x y _ => add (natToInt x) (natToInt y) .int
-    | mul x y _ => mul (natToInt x) (natToInt y) .int
-    | div x y _ => div (natToInt x) (natToInt y) .edivInt
-    | mod x y _ => mod (natToInt x) (natToInt y) .edivInt
-    | var _ | sub _ _ _ | neg _ | intToNat _ | natToInt _ => v)
+    | add x y _ => simp <| add (natCast x) (natCast y) .int
+    | mul x y _ => simp <| mul (natCast x) (natCast y) .int
+    | div x y _ => simp <| div (natCast x) (natCast y) .edivInt
+    | mod x y _ => simp <| mod (natCast x) (natCast y) .edivInt
+    | var _ | sub .. | neg _ | natCast _
+      | eq .. | le .. | lt .. | true | false => v)
   | add x y tp =>
     match x, y with
     | x, lit 0 _ => x
@@ -152,6 +181,8 @@ partial def simp (v : NumTerm) : NumTerm :=
     | lit 0 _, y, .int => simp (neg y)
     | x, y, _ => Id.run <| do
       match tp with
+      | .prop =>
+        panic! "sub applied to prop"
       | .nat =>
         if let (lit xo _, lit yo _) := (x, y) then
           return lit (xo - yo) .nat
@@ -292,27 +323,80 @@ partial def simp (v : NumTerm) : NumTerm :=
         if xa == n || xb == n then
           return lit 0 tp
       if let mod xn xd xop := x then
-        if xd == n then
-          let rop :=
-            match op, xop with
-            | .divNat, .divNat => some .divNat
-            | .edivInt, _ => some .edivInt
-            | .tdivInt, .edivInt => some .edivInt
-            | .tdivInt, .tdivInt => some .tdivInt
-            | .fdivInt, .edivInt => some .fdivInt
-            | .fdivInt, .fdivInt => some .fdivInt
-            | .bdivInt, _ => some .bdivInt
-            | _, _ => none
-          if let some rop := rop then
-            return simp (mod xn n rop)
+        let rop : Option NumTerm :=
+          match op, xop with
+          | .divNat,  .divNat  => do guard (n == xd); some (mod xn n .divNat)
+          | .edivInt, .bdivInt => do guard (n == natCast xd); some (mod xn n .edivInt)
+          | .edivInt, _        => do guard (n == xd); some (mod xn n .edivInt)
+          | .tdivInt, .edivInt => do guard (n == xd); some (mod xn n .edivInt)
+          | .tdivInt, .tdivInt => do guard (n == xd); some (mod xn n .tdivInt)
+          | .fdivInt, .edivInt => do guard (n == xd); some (mod xn n .fdivInt)
+          | .fdivInt, .fdivInt => do guard (n == xd); some (mod xn n .fdivInt)
+          | .bdivInt, .bdivInt => do guard (n == xd); some (mod xn n .bdivInt)
+          | .bdivInt, _        => do guard (natCast n == xd); some (mod xn n .bdivInt)
+          | _, _ => none
+        if let some r := rop then
+            return simp r
       if let neg yn := n then
         match op with
-        | .edivInt | .tdivInt | .bdivInt =>
+        | .edivInt | .tdivInt =>
           return simp (mod x yn op)
         | _ =>
           pure ()
       return v
-  | _ => v
+  | eq x y _ => Id.run do
+      if let (some i, some j) := (asIntLit x, asIntLit y) then
+        return mkConstProp (i = j)
+      if x == y then
+        return NumTerm.true
+      pure v
+  | le x y _ => Id.run do
+      if let (some i, some j) := (asIntLit x, asIntLit y) then
+        return mkConstProp (i ≤ j)
+--      if let (some xn, some yn) := (intAtNat x, intAtNat y) then
+--        return (le xn yn .nat)
+      if x == y then
+        return NumTerm.true
+      pure v
+  | lt x y tp => Id.run do
+      if let (some i, some j) := (asIntLit x, asIntLit y) then
+        return mkConstProp (i < j)
+      if let (lit 0 .int, natCast yn) := (x, y) then
+        return simp (lt (lit 0 .nat) yn .nat)
+      if let (natCast xn, natCast yn) := (x, y) then
+        return simp (lt xn yn .nat)
+      if tp = .nat then
+        if x == y then
+          return NumTerm.false
+        if let add yb (lit yo _) _ := y then
+          if x == yb then
+            return mkConstProp (yo > 0)
+        if let (lit xo _, add yb (lit yo _) _) := (x, y) then
+          let r := if xo < yo then NumTerm.true else lt (lit (xo - yo) .nat) yb .nat
+          return r
+        if let (add xb (lit xo _) _, lit yo _) := (x, y) then
+          let r :=
+            if xo < yo then
+              lt xb (lit (yo - xo) .nat) .nat
+            else
+              NumTerm.false
+          return r
+        if let (add xb (lit xo _) _, add yb (lit yo _) _) := (x, y) then
+          let r :=
+            if xo < yo then
+              lt xb (add yb (lit (yo - xo) .nat) .nat) .nat
+            else if xo > yo then
+              lt (add xb (lit (xo - yo) .nat) .nat) yb .nat
+            else
+              lt xb yb .nat
+          return r
+        if let (lit 0 _, mul y1 y2 _) := (x, y) then
+          if isPos y1 then
+            return lt (lit 0 nat) y2 nat
+          if isPos y2 then
+            return lt (lit 0 nat) y1 nat
+      pure v
+  | true | false | lit _ _ | var _ => v
 
 partial def simpv (u : NumTerm) : NumTerm :=
   let v := simp u
@@ -322,12 +406,14 @@ partial def simpv (u : NumTerm) : NumTerm :=
     panic! s!"simp result changed types:\n  Input: {repr u}\n  Out:   {repr v}"
 
 def litOp (n : Nat) (tp : NumType) := mkOp [] tp fun _ => lit n tp
-def addOp (tp : NumType) := mkOp [tp, tp] tp fun a => add (a[0]!) (a[1]!) tp
-def subOp (tp : NumType) := mkOp [tp, tp] tp fun a => sub (a[0]!) (a[1]!) tp
+def binOp (op : NumTerm → NumTerm → NumType → NumTerm) (tp : NumType) :=
+  mkOp [tp, tp] tp fun a => op (a[0]!) (a[1]!) tp
+def binRel (op : NumTerm → NumTerm → NumType → NumTerm) (tp : NumType) :=
+  mkOp [tp, tp] .prop fun a => op (a[0]!) (a[1]!) tp
 def negOp : Op NumType NumTerm := mkOp [.int] .int fun a => neg (a[0]!)
-def mulOp (tp : NumType) := mkOp [tp, tp] tp fun a => mul (a[0]!) (a[1]!) tp
 def divOp (op : DivMode) (dtp := op.typeOf) := let tp := op.typeOf; mkOp [tp, dtp] tp fun a => div (a[0]!) (a[1]!) op
 def modOp (op : DivMode) (dtp := op.typeOf) := let tp := op.typeOf; mkOp [tp, dtp] tp fun a => mod (a[0]!) (a[1]!) op
+def natToIntOp := mkOp [NumType.nat] .int fun x => natCast x[0]!
 
 end NumTerm
 
@@ -337,7 +423,7 @@ syntax:lead (name := intTestElab) "#intTest" : command
 
 @[command_elab intTestElab]
 def elabIntTest : CommandElab := fun _stx => do
-  let types : List NumType := [.nat, .int]
+  let types : List NumType := [.prop, .nat, .int]
   let ops := [
       litOp 0 .nat,
       litOp 1 .nat,
@@ -345,12 +431,16 @@ def elabIntTest : CommandElab := fun _stx => do
       litOp 0 .int,
       litOp 1 .int,
       litOp 2 .int,
-      addOp .nat, addOp .int,
-      subOp .nat, subOp .int,
+      natToIntOp,
+      binOp add .nat, binOp add .int,
+      binOp sub .nat, binOp sub .int,
+      binOp mul .nat, binOp mul .int,
       negOp,
-      mulOp .nat, mulOp .int,
       divOp .divNat, divOp .edivInt, divOp .fdivInt, divOp .tdivInt, divOp .bdivInt .nat,
       modOp .divNat, modOp .edivInt, modOp .fdivInt, modOp .tdivInt, modOp .bdivInt .nat,
+      binRel eq .nat, binRel eq .int,
+      binRel le .nat, binRel le .int,
+      binRel lt .nat, binRel lt .int,
   ]
   let vars : List (NumType × CoreM Command) := [
       (.nat, `(variable (n : Nat))),
@@ -359,5 +449,74 @@ def elabIntTest : CommandElab := fun _stx => do
   let stats : GenStats := { maxTermSize := 6, maxDepth := 3, maxVarCount := 2 }
   testNormalForms types ops vars NumTerm.simpv stats
 
+set_option pp.coercions false
+set_option pp.explicit true
 set_option maxHeartbeats 100000000
 #intTest
+
+variable (m n : Nat)
+
+/-
+
+  @LT.lt Nat instLTNat (@OfNat.ofNat Nat 1 (instOfNatNat 1))
+    (@HAdd.hAdd Nat Nat Nat (@instHAdd Nat instAddNat) n0 (@OfNat.ofNat Nat 2 (instOfNatNat 2))) reduces to
+  @LT.lt Nat instLTNat (@OfNat.ofNat Nat 1 (instOfNatNat 1))
+    (@HAdd.hAdd Nat Nat Nat (@instHAdd Nat instAddNat) n0 (@OfNat.ofNat Nat 2 (instOfNatNat 2)))
+but is expected to reduce to
+  True
+
+-/
+
+set_option trace.Meta.Tactic.simp.rewrite true
+
+#check_tactic n < n + 1 ~> True by simp
+
+#check_tactic 0 < n + 2 ~> True by
+  simp
+
+#check_simp 1 < n + 2 !~>
+
+
+#print Nat.mul_pos_iff_of_pos_left
+#check_tactic 0 < n + 2 ~> True by simp
+
+#check_tactic 0 < 2 * n ~> 0 < n by simp
+
+
+
+#check_tactic (@OfNat.ofNat Int 0 (@instOfNat 0)) < (@Nat.cast Int _ n0) ~> m < n by
+  simp
+
+set_option trace.Meta.Tactic.simp.rewrite true
+
+#print Int.ofNat_pos
+
+#check_tactic ((0 : Int) < @Nat.cast Int _ n) ~> 0 < n by
+  simp
+
+
+#check_simp ((1 : Int) < @Nat.cast Int _ n) !~> 1 < n.cast
+
+#check_tactic ((0 : Int) < (n : Int)) ~> 0 < n by
+  simp
+
+
+--set_option pp.notation fals
+
+example : ((1 : Nat) < (n : Int)) := by
+  simp
+
+#check_tactic ((1 : Nat) < (n : Int)) ~> 1 < n by
+  simp
+
+#check_tactic (n < n + 2) ~> True by
+  simp
+
+
+
+--#check_tactic (1 < (n : Int)) ~> 1 < n by
+--  simp
+
+/-
+
+-/
