tests/lean/run/simprocNat.lean
@@ -41,7 +41,7 @@ variable (a b : Nat)
 #check_simp (1234567 : Nat) ≠ 123456 ~> True
 #check_simp (a + 400) ≠ (b + 1000) ~> a ≠ b + 600
 
-/- leq -/
+/- le -/
 
 #check_simp (1234567 : Nat) ≤ 123456 ~> False
 #check_simp (1234567 : Nat) ≤ 1234567 ~> True
@@ -67,6 +67,36 @@ variable (a b : Nat)
 #check_simp (a +  400) ≥ 1000 ~> a ≥ 600
 #check_simp 1000 ≥ (a + 1000) ~> a = 0
 #check_simp (a + 1000) ≥ (b +  400) ~> a + 600 ≥ b
+
+/- lt -/
+
+#check_simp (1234567 : Nat) < 123456 ~> False
+#check_simp (1234567 : Nat) < 1234567 ~> False
+#check_simp (1234567 : Nat) < 1234568 ~> True
+#check_simp (123456 : Nat) < 1234567 ~> True
+
+#check_simp (a +  999) < 1000 ~> a < 1
+#check_simp (a + 1000) < 1000 ~> False
+#check_simp (a + 1000) <  400 ~> False
+#check_simp (a +  400) < 1000 ~> a < 600
+
+#check_simp 1000 < (a + 1000) ~> 0 < a
+#check_simp 400  < (a + 1000) ~> True
+#check_simp 1000 < (a +  400) ~> 600 < a
+
+#check_simp (a +  999) < (b + 1000) ~> a < b + 1
+#check_simp (a + 1000) < (b + 1000) ~> a < b
+#check_simp (a + 1000) < (b +  400) ~> a + 600 < b
+#check_simp (a +  400) < (b + 1000) ~> a < b + 600
+#check_simp (Nat.add a 400) < (Add.add b 1000) ~> a < b + 600
+#check_simp (Nat.add a 400) < b.succ.succ ~> a + 398 < b
+
+/- gt (just make sure lt rules apply) -/
+
+#check_simp (123456 : Nat) > 1234567 ~> False
+#check_simp (a +  400) > 1000 ~> a > 600
+#check_simp 1000 > (a + 1000) ~> False
+#check_simp (a + 1000) > (b +  400) ~> a + 600 > b
 
 /- beq tests -/
 
